ch26-max-flow/CLRS.Ch26.MaxFlow.Test.fst
@@ -42,7 +42,7 @@ fn test_max_flow_example ()
   assume_ (pure (valid_caps sc2 (SZ.v n)));
   
   // Run max flow algorithm
-  max_flow capacity flow n 0sz 2sz;
+  let _valid = max_flow capacity flow n 0sz 2sz;
   
   // Clean up
   with sc. assert (A.pts_to capacity sc);
